Games/games/PickUpBricks.lean
@@ -1,0 +1,116 @@
+/-
+Copyright (c) 2024 Yves Jäckle. All rights reserved.
+Released under Apache 2.0 license as described in the file LICENSE.
+Author: Yves Jäckle.
+-/
+
+import Games.gameLib.Termination
+import Games.gameLib.HistoryAPI
+
+
+variable (init_bricks : ℕ) -- the initial number of bricks as a variable
+
+/--
+Given an initial number of bricks and a history of bricks taken, return the current number of bricks.
+-/
+def bricks_from_ini_hist (ini : ℕ) (hist : List ℕ) := ini - hist.sum
+
+/--
+Given an initial number of bricks, a history of bricks taken and the current number of bricks
+being taken, return the current number of bricks.
+-/
+def bricks_from_ini_hist_act (ini : ℕ) (hist : List ℕ) (act : ℕ) := ini - hist.sum - act
+
+
+lemma bricks_cons (ini : ℕ) (hist : List ℕ) (x : ℕ) :
+  bricks_from_ini_hist ini (x :: hist) = bricks_from_ini_hist ini hist - x :=
+  by
+  dsimp [bricks_from_ini_hist]
+  rw [List.sum_cons]
+  rw [add_comm, Nat.sub_add_eq]
+
+
+def PickUpBricks : Symm_Game_World ℕ ℕ where
+  init_game_state := init_bricks
+  fst_win_states := (fun hist => bricks_from_ini_hist init_bricks hist = 0) -- won once no bricks left
+  snd_win_states := (fun hist => bricks_from_ini_hist init_bricks hist = 0)
+  transition :=  bricks_from_ini_hist_act init_bricks
+  law := fun hist act =>  let B := (bricks_from_ini_hist init_bricks hist)
+                              if B = 0
+                              then act = 0
+                              else  if B = 1
+                                    then act = 1
+                                    else act = 1 ∨ act = 2
+
+instance : DecidablePred (PickUpBricks init_bricks).fst_win_states := by
+  intro hist
+  dsimp [PickUpBricks, bricks_from_ini_hist]
+  exact Nat.decEq (init_bricks - List.sum hist) 0
+
+instance : DecidablePred (PickUpBricks init_bricks).snd_win_states := by
+  intro hist
+  dsimp [PickUpBricks, bricks_from_ini_hist]
+  exact Nat.decEq (init_bricks - List.sum hist) 0
+
+
+
+def pub_win_strat : (PickUpBricks init_bricks).sStrategy :=
+  fun hist _ _ =>
+    let B := bricks_from_ini_hist init_bricks hist
+    if Z : B = 0
+    then ⟨0, (by dsimp [PickUpBricks] ; dsimp [B] at Z ; rw [Z, if_pos rfl])⟩
+    else  if M : B % 3 = 1
+          then ⟨1, (by dsimp [PickUpBricks] ; dsimp [B] at Z M ; rw [if_neg Z] ; split_ifs ; rfl ; left ; rfl)⟩
+          else ⟨2, (by dsimp [PickUpBricks] ; dsimp [B] at Z M ; rw [if_neg Z] ; rw [if_neg (by contrapose! M ; rw [M] ; decide)] ; right ; rfl )⟩
+
+
+def toy_strat : (PickUpBricks init_bricks).fStrategy :=
+  fun hist _ _ =>
+    let B := bricks_from_ini_hist init_bricks hist
+    if Z : B = 0
+    then ⟨0, (by dsimp [PickUpBricks] ; dsimp [B] at Z ; rw [Z, if_pos rfl])⟩
+    else ⟨1, (by dsimp [PickUpBricks] ; dsimp [B] at Z ; rw [if_neg Z] ; split_ifs ; rfl ; left ; rfl)⟩
+
+
+/--
+Pick up bricks played with 32 initial bricks, with the winning strat as
+first strat and the toy strat as second strat
+-/
+def PickUpBricks_pubWin_vs_toy : Symm_Game ℕ ℕ :=
+  {(PickUpBricks 37) with
+   fst_strat := toy_strat 37
+   snd_strat := pub_win_strat 37
+  }
+
+
+instance : DecidablePred (PickUpBricks_pubWin_vs_toy).fst_win_states := by
+  intro hist
+  dsimp [PickUpBricks_pubWin_vs_toy]
+  apply instDecidablePredListNatFst_win_statesPickUpBricks
+
+instance : DecidablePred (PickUpBricks_pubWin_vs_toy).snd_win_states := by
+  intro hist
+  dsimp [PickUpBricks_pubWin_vs_toy]
+  apply instDecidablePredListNatFst_win_statesPickUpBricks
+
+
+#eval (PickUpBricks_pubWin_vs_toy.hist_on_turn 30).val.reverse
+#eval (List.range 30).map (PickUpBricks_pubWin_vs_toy.state_on_turn)
+
+
+lemma loop_invariant
+  (win_hyp : 3 ∣ init_bricks)
+  (f_strat : (PickUpBricks init_bricks).fStrategy) :
+  let g : Symm_Game ℕ ℕ := { (PickUpBricks init_bricks) with
+                             fst_strat := f_strat
+                             snd_strat := pub_win_strat init_bricks
+                            } ;
+  ∀ turn, Turn_snd turn → 3 ∣ bricks_from_ini_hist init_bricks (g.hist_on_turn turn) :=
+  by
+  intro g t T
+  apply Invariant_snd _ _ t T
+  · dsimp [bricks_from_ini_hist, Symm_Game.hist_on_turn, Symm_Game_World.hist_on_turn, Game_World.hist_on_turn]
+    exact win_hyp
+  · intro t T ih
+    rw [Symm_Game.hist_on_turn, Symm_Game_World.hist_on_turn_2step_snd _ _ _ T, bricks_from_ini_hist]
+    rw [List.sum_cons, List.sum_cons]
